Flesh out LeastFixedPoint.v

src/LeastFixedPoint.v
@@ -7,7 +7,67 @@ Require Import Coq.Classes.Morphisms.
 Require Export InformationOrdering.
 Open Scope code_scope.
 
-Lemma Y_lfp (Var : Set) (f b : Code Var) :
+Fixpoint power {Var : Set} (f : Code Var) (n : nat) : Code Var :=
+  match n with
+  | 0 => I
+  | Succ n' => f o (power f n')
+  end.
+
+Notation "f ^ n" := (power f n) : code_scope.
+
+Lemma power_0 (Var : Set) (f x : Code Var) : f ^ 0 * x == x.
+Proof. simpl; beta_simpl; auto. Qed.
+
+Lemma power_1 (Var : Set) (f x : Code Var) : f ^ 1 * x == f * x.
+Proof. simpl; beta_simpl; auto. Qed.
+
+Lemma power_2 (Var : Set) (f x : Code Var) : f ^ 2 * x == f * (f * x).
+Proof. simpl; beta_simpl; auto. Qed.
+
+Lemma Y_limit_ub (Var : Set) (f : Code Var) (n : nat) : f ^ n * BOT [= Y * f.
+Proof.
+  induction n.
+    simpl; beta_simpl; auto.
+  unfold power; fold (@power Var); rewrite beta_b.
+  rewrite beta_y; monotonicity.
+Qed.
+
+Lemma Y_limit_lb
+  (Var : Set) (f : Code Var)
+  (Var' : Set) (c : Code Var') (b : Var -> Code Var') :
+  conv (c * (Y * f @ b)) -> exists n, conv (c * (f ^ n * BOT @ b)).
+Proof.
+  (* sketch: prove the only beta path from [Y * f] to [f ...] is [beta_y]. *)
+Admitted.
+
+Lemma Y_limit_lub (Var : Set) (f x : Code Var) :
+  (forall n : nat, f ^ n * BOT [= x) -> Y * f [= x.
+Proof.
+  unfold code_le; intros Hl Var' c b Hc.
+  apply Y_limit_lb in Hc as [n Hn]; eauto.
+Qed.
+
+Lemma Y_fp (Var : Set) (f : Code Var) : Y * f == f * (Y * f).
+Proof.
+  rewrite <- beta_y; reflexivity.
+Qed.
+
+Lemma Y_lfp (Var : Set) (f x : Code Var) : f * x [= x -> Y * f [= x.
+Proof.
+  intro Hl.
+  assert (forall n : nat, f ^ n * BOT [= x).
+    induction n.
+      simpl; beta_simpl; auto.
+    unfold power; fold (@power Var); rewrite beta_b.
+    rewrite <- Hl; monotonicity.
+  apply Y_limit_lub; auto.
+Qed.
+
+Lemma Y_ub (Var : Set) (f b : Code Var) :
   (forall x, x [= b -> f * x [= b) -> Y * f [= b.
+Proof.
+Admitted.
+
+Lemma Y_ident (Var : Set) (y : Code Var) : y == S * I * y -> y = Y.
 Proof.
 Admitted.
